common/SkelInfo.v
@@ -8,11 +8,18 @@ Set Implicit Arguments.
 Local Set Elimination Schemes.
 Local Set Case Analysis Schemes.
 
-Definition skel_le (sk1 sk2: AST.program unit unit): Prop :=
-  (forall id g, (prog_defmap sk1) ! id = Some g -> (prog_defmap sk2) ! id = Some g)
-  /\ (forall id g, (prog_defmap sk2)! id = Some g -> In id (prog_public sk2) ->
-             (prog_defmap sk1)! id = Some g)
-  /\ (prog_public sk2 = prog_public sk1).
+Record skel_prop (sk: AST.program unit unit): Prop := {
+    public_defined: forall id, In id (prog_public sk) -> AST.has_symbol sk id;
+    main_public: In (prog_main sk) (prog_public sk);
+  }.
+
+Record skel_le (sk1 sk2: AST.program unit unit): Prop := {
+    defmap_le: forall id g, (prog_defmap sk1) ! id = Some g -> (prog_defmap sk2) ! id = Some g;
+    defmap_public: forall id g, (prog_defmap sk2)! id = Some g -> In id (prog_public sk2) ->
+            (prog_defmap sk1)! id = Some g;
+    public_same: prog_public sk2 = prog_public sk1;
+    main_same: prog_main sk2 = prog_main sk1;
+  }.
 
 Instance skel_le_refl: Reflexive skel_le.
 Proof.
@@ -21,12 +28,10 @@ Qed.
 
 Instance skel_le_tran: Transitive skel_le.
 Proof.
-  intros sk1 sk2 sk3 [H11 [H12 H13]] [H21 [H22 H23]].
-  split.
-  intros. eauto.
-  split.
-  intros. eapply H12; eauto. rewrite <- H23. eauto.
-  congruence.
+  intros sk1 sk2 sk3 H1 H2. destruct H1. destruct H2.
+  split; try congruence; intros; eauto.
+  eapply defmap_public0; eauto.
+  rewrite <- public_same1; eauto.
 Qed.
 
 Record match_stbls' (f: meminj) (ge1: Genv.symtbl) (ge2: Genv.symtbl) := {
@@ -63,11 +68,54 @@ Inductive match_stbls_static (kept: ident -> Prop) (removed: ident -> Prop)
       forall id, Genv.has_symbol ge2 id -> Genv.has_symbol ge1 id;
   }.
 
+(* Because public symbols must be preserved, we only care about the static
+   symbols. But when [skel_info] is used together with [skel_le], we can infer
+   that removed symbols are static. So sometimes we don't separate public and
+   static symbols in [skel_info] *)
 Inductive skel_info :=
   | Atom (kept: ident -> Prop) (removed: ident -> Prop): skel_info
   | Compose (info1 info2: skel_info): skel_info.
 
 Definition atom_skel_info (sk: AST.program unit unit) :=
-  Atom (fun id => AST.has_symbol sk id /\ ~ In id sk.(prog_public)) (fun _ => False).
+  Atom (fun id => AST.has_symbol sk id) (fun _ => False).
 
 Definition skel := AST.program unit unit.
+
+Inductive skel_info_le: skel_info -> skel_info -> Prop :=
+  | skel_info_le_atom (kept1 kept2 removed1 removed2: ident -> Prop):
+    (forall id, kept1 id -> kept2 id) ->
+    (forall id, removed1 id -> removed2 id) ->
+    skel_info_le (Atom kept1 removed1) (Atom kept2 removed2)
+  | skel_info_le_compose info1 info2 info1' info2':
+    skel_info_le info1 info1' ->
+    skel_info_le info2 info2' ->
+    skel_info_le (Compose info1 info2) (Compose info1' info2').
+
+Instance skel_info_le_refl: Reflexive skel_info_le.
+Proof.
+  intro skel_info. induction skel_info; constructor; easy.
+Qed.
+
+Instance skel_info_le_tran: Transitive skel_info_le.
+Proof.
+  intros si1 si2 si3 H12 H23.
+  revert si3 H23. induction H12.
+  - intros. inv H23. constructor; firstorder.
+  - intros. inv H23.
+    specialize (IHskel_info_le1 _ H1).
+    specialize (IHskel_info_le2 _ H3).
+    constructor; eauto.
+Qed.
+
+Lemma linkorder_skel_info_le sk1 sk2:
+  linkorder sk1 sk2 ->
+  skel_info_le (atom_skel_info sk1) (atom_skel_info sk2).
+Proof.
+  intros (Hmain & Hpub & Hdefs). constructor. 2: easy.
+  intros id Hid1. unfold has_symbol in *.
+  exploit prog_defmap_dom; eauto. intros (g & Hg).
+  specialize (Hdefs _ _ Hg) as (g' & Hg' & ? & ?).
+  apply in_prog_defmap in Hg'.
+  unfold prog_defs_names.
+  eapply in_map with (f:=fst) in Hg'. apply Hg'.
+Qed.
